Interface.v
@@ -1,17 +1,25 @@
 Require Import lib.Integers.
 Require Import Rustre.Common.
+Require Import common.Smallstep.
+Require Import common.Events.
+Require Import common.Globalenvs.
+Require Import common.Memory.
+Require Import Rustre.Minimp.Syntax.
+Require Import Rustre.Minimp.Semantics.
 
 (* Interface avec CompCert *)
 Inductive val' : Type :=
 | Vundef : val'
-| Vint : Int.int -> val'. 
+| Vint : Int.int -> val'.
+
 Inductive unary_op' : Type :=
 | Opposite : unary_op'
 | Negation : unary_op'.
+
 Inductive binary_op' : Type :=
-| Plus : binary_op'
-| Minus : binary_op'
-| Mult : binary_op'.
+| Add : binary_op'
+| Sub : binary_op'
+| Mul : binary_op'.
 
 Definition zero := Int.zero.
 Definition one := Int.one.
@@ -62,9 +70,9 @@ Module Op <: OPERATORS.
   
   Definition sem_binary (op : binary_op) (v1 v2 : val) : option val :=
     match op with
-    | Plus => sem_plus v1 v2
-    | Minus => sem_minus v1 v2
-    | Mult => sem_mult v1 v2
+    | Add => sem_plus v1 v2
+    | Sub => sem_minus v1 v2
+    | Mul => sem_mult v1 v2
     end.
 
   Definition of_bool (b : bool) : val := Vint (if b then Int.one else Int.zero).
@@ -129,3 +137,44 @@ Module Op <: OPERATORS.
   Proof. intros op1 op2; unfold binop_eqb; destruct (binop_dec op1 op2); intuition. Qed.
 
 End Op.
+
+Module Import Syn := SyntaxFun Op.
+Module Import Sem := SemanticsFun Op Syn.
+
+Record fundeft := Fundeft {name: ident; body: stmt}.
+Parameter vart: Type.
+Parameter pub: program -> list ident.
+Parameter def: program -> list (ident * AST.globdef fundeft vart).
+
+Definition genv := Genv.t fundeft vart.
+Inductive state :=
+| State (H: heap) (S: stack) (s: stmt)
+| StopState.
+Parameter convert_prog: program -> AST.program fundeft vart.
+
+Inductive step: genv -> state -> trace -> state -> Prop :=
+| DoStep: forall prog ge H S s H' S' t,
+    stmt_eval prog H S s (H', S') ->
+    step ge (State H S s) t (State H' S' Skip)
+| Stop: forall ge H S t,
+    step ge (State H S Skip) t StopState.
+
+Parameter convert_mem: mem -> heap * stack.
+Inductive initial_state (ge : genv) (p: program): state -> Prop :=
+  IniState: forall b f m0 H0 S0,
+    let p' := convert_prog p in
+    Genv.init_mem p' = Some m0 ->
+    Genv.find_symbol ge p'.(AST.prog_main) = Some b ->
+    Genv.find_funct_ptr ge b = Some f ->
+    convert_mem m0 = (H0, S0) ->
+    initial_state ge p (State H0 S0 f.(body)).
+
+Inductive final_state: state -> int -> Prop :=
+  FinalState: final_state StopState zero.
+
+Definition globalenv (p: program) :=
+  Genv.globalenv (convert_prog p).
+
+Definition semantics (p: program) :=
+  let ge := globalenv p in
+  Semantics_gen step (initial_state ge p) final_state ge ge.
